\documentclass{jsarticle}
\begin{document}

\section{}

\subsection{} % subsection1
\begin{eqnarray*}
	gh 
	&=& (1 - 2\sigma_2 + 3\sigma_5)(3\sigma_6 - 2\sigma_4 + \sigma_2)\\
	&=& (3\sigma_6 - 2\sigma_4 + \sigma_2) - 2\sigma_2(3\sigma_6 - 2\sigma_4 + \sigma_2) + 3\sigma_5(3\sigma_6 - 2\sigma_4 + \sigma_2)\\
	&=& (3\sigma_6 - 2\sigma_4 + \sigma_2) - (6\sigma_3 - 4\sigma_5 + 2\sigma_1) + (9\sigma_1 - 6\sigma_2 + 3\sigma_3)\\
	&=& 7 - 5\sigma_2 - 3\sigma_3 - 2\sigma_4 + 4\sigma_5 + 3\sigma_6
\end{eqnarray*}

\subsection{} % subsection2
$h, h' \in G \subset A[G]$に対して$gh = gh'$とすると$h = h'$なので, $gN = \sum_{h \in G}gh = \sum_{h \in G}h = N$である. $Ng = N$も同様に示される.

\subsection{} % subsection3
$2a + b = 4 + 5\sqrt{-2}$, $ab = 8 + 5\sqrt{-2}$

\section{}
\subsection{} % subsection1


\subsection{} % subsection2
\subsection{} % subsection3
\subsection{} % subsection4
\subsection{} % subsection5

\subsection{} % subsection1
\subsection{} % subsection2
\subsection{} % subsection2
\subsection{} % subsection2
\subsection{} % subsection2
\subsection{} % subsection2
\subsection{} % subsection2
\subsection{} % subsection2
\subsection{} % subsection2
\subsection{} % subsection2
\subsection{} % subsection2
\subsection{} % subsection2
\subsection{} % subsection2
\subsection{} % subsection2
\subsection{} % subsection2
\subsection{} % subsection2
\subsection{} % subsection2
\subsection{} % subsection2
\subsection{} % subsection2
\subsection{} % subsection2
\subsection{} % subsection2
\subsection{} % subsection2
\subsection{} % subsection2

\end{document}